theories/Escape.v
@@ -2,190 +2,71 @@ From MetaCoq Require Import PCUICAst.
 Require Import Automation Untyped MLTTTyping LogicalRelation Properties Reduction LRInduction.
 Set Universe Polymorphism.
 
-Definition escape0 {Γ A} :
-    [Γ ||-< zero | A ] ->
+Definition escape {l Γ A} :
+    [Γ ||-< l > A ] ->
     [Γ |- A].
 Proof.
-  destruct 1.
-  eapply (LR_rect0 (fun Γ A _ _ _ _ => [Γ |- A])).
-  3: eassumption.
-  - intros ? ? neA.
-    now destruct neA as [? []].
-  - intuition.
-Qed.
-
-Definition escape1 {Γ A} :
-    [Γ ||-< one | A ] ->
-    [Γ |- A].
-Proof.
-  intros [? ? ? valid].
-  red in valid ; cbn in *.
-  eapply (LR_rect1' (fun Γ A _ _ _ _ => [Γ |- A]) (fun Γ A _ _ _ _ => [Γ |- A])).
-  6: eassumption.
-  - intros.
-    eapply escape0.
-    logrel.
+  eapply (LR_rect (fun l Γ A _ => [Γ |- A])).
   - intros ? [].
     mltt.
-  - intros ? ? [].
-    now destruct red.
-  - intros ? ? [].
-    now destruct red.
-  - easy.
+  - intros _ ? ? [] ; cbn in *.
+    mltt.
+  - intros ? ? ? [] ; cbn in *.
+    mltt.
 Qed.
 
-Definition escapeEqNe {Γ0 A0 B} : forall (neA : [Γ0 ||-ne A0]),
-    [Γ0 ||-ne A0 ≅ B | neA] ->
-    [Γ0 |- A0 ≅ B].
+Definition escapeEq {l Γ A B} (lr : [Γ ||-< l > A]) :
+    [ Γ ||-< l > A ≅ B | lr ] ->
+    [Γ |- A ≅ B].
 Proof.
-    intros [] [] ; cbn in *.
+  eapply (LR_rect (fun l Γ A lr => forall B : term, [Γ ||-< l > A ≅ B | lr] -> [Γ |- A ≅ B])).
+  + intros ? [] ? [->].
+    mltt.
+  + intros ? ? ? [] ? [].
+    do 2 eapply TypeTrans.
+    all: mltt.
+  + intros ? ? ? [] _ _ _ ? [] ; cbn in *.
     do 2 eapply TypeTrans.
     all: mltt.
 Qed.
 
-Definition escapeEqPi {Γ A} : forall (ΠA : [Γ ||-Πr A]),
-    forall B, [Γ ||-Π A ≅ B | ΠA] -> [Γ |- A ≅ B].
+Definition escapeTerm {l Γ t A} (lr : [Γ ||-< l > A ]) :
+  [Γ ||-< l > t : A | lr ] ->
+  [Γ |- t : A].
 Proof.
-  intros [] ? [].
-  do 2 eapply TypeTrans.
-  all: mltt.
+  eapply (LR_rect (fun l Γ A lr => forall t : term, [Γ ||-< l > t : A | lr ] -> [Γ |- t : A])).
+  - intros ? [] ? [] ; cbn in *.
+    mltt.
+  - intros ? ? ? [] ? [] ; cbn in *.
+    mltt.
+  - intros ? ? ? [] _ _ _ ? [] ; cbn in *.
+    mltt.
 Qed.
 
-Definition escapeEq0 {Γ A B} (H : [Γ ||-< zero | A]) :
-    [ Γ ||-< zero | A ≅ B | H ] ->
-    [Γ |- A ≅ B].
+Definition escapeEqTerm {l Γ t u A} (lr : [Γ ||-< l > A ]) :
+  [Γ ||-< l > t ≅ u : A | lr ] ->
+  [Γ |- t ≅ u: A].
 Proof.
-  eapply (LR_rect0
-    (fun Γ A T T0 T1 H => forall B : term,
-      [Γ ||-< zero | A ≅ B | Build_LRValid H] -> 
-      [Γ |- A ≅ B])).
-  + intros; now eapply escapeEqNe. 
-  + intros; now eapply escapeEqPi.
-Qed.
-
-Definition escapeEq1 {Γ A B} (H : [Γ ||-< one | A]) :
-    [ Γ ||-< one | A ≅ B | H ] ->
-    [Γ |- A ≅ B].
-Proof.
-    eapply (LR_rect1'
-      (fun Γ A T T0 T1 H => forall B : term,
-        [Γ ||-< zero | A ≅ B | Build_LRValid H] -> 
-        [Γ |- A ≅ B])
-    (fun Γ A T T0 T1 H => forall B : term,
-        [Γ ||-< one | A ≅ B | Build_LRValid H] -> 
-        [Γ |- A ≅ B])). 
-    all: cbn in *.
-    - intros.
-      now eapply (escapeEq0 (LRbuild lr)).
-    - intros ? [] _ [->].
-      mltt.
-    - intros ? ? [] ? [] ; cbn in *.
-      do 2 eapply TypeTrans.
-      all: mltt.
-    - intros.
-      now eapply escapeEqPi.
-    - eauto.
-Qed.
-
-Definition escapeTermNe {Γ0 A0 t}: forall
-  (neA : [Γ0 ||-ne A0]),
-  [Γ0 ||-ne t ::: A0 | neA] -> 
-  [Γ0 |- t ::: A0].
-Proof.
-  intros [] [? []] ; cbn in *.
-  mltt.
-Qed.
-
-Definition escapeTermPi {Γ A} : forall (ΠA : [Γ ||-Πr A]) (t : term), 
-  [Γ ||-Π t ::: A | ΠA] -> 
-  [Γ |- t ::: A].
-Proof.
-  intros [? ? ? ? []] ? [? []]; cbn in *.
-  mltt.
-Qed.
-
-Definition escapeTerm0 {Γ t A} (H : [Γ ||-< zero | A ]) :
-  [Γ ||-< zero | t ::: A | H ] ->
-  [Γ |- t ::: A].
-Proof.
-  eapply (LR_rect0
-    (fun Γ A T T0 T1 H => forall t : term,
-      [Γ ||-< zero | t ::: A | Build_LRValid H] -> 
-      [Γ |- t ::: A])).
-  all: eauto using escapeTermNe, escapeTermPi.
-Qed.
-
-Definition escapeTerm1 {Γ t A} (H : [Γ ||-< one | A ]) :
-  [Γ ||-< one | t ::: A | H ] ->
-  [Γ |- t ::: A].
-Proof.
-  eapply (LR_rect1'
-    (fun Γ A T T0 T1 H => forall t : term,
-      [Γ ||-< zero | t ::: A | Build_LRValid H] -> 
-      [Γ |- t ::: A])
-      (fun Γ A T T0 T1 H => forall t : term,
-      [Γ ||-< one | t ::: A | Build_LRValid H] -> 
-      [Γ |- t ::: A])).
-  all: cbn.
-  - intros.
-    now eapply (escapeTerm0 (LRbuild lr)).
-  - intuition.
-  - eauto using escapeTermNe.
-  - eauto using escapeTermPi.
-  - auto.
-Qed.
-
-Definition escapeEqTermNe {Γ0 A0 t u}: forall
-  (neA : [Γ0 ||-ne A0]),
-  [Γ0 ||-ne t ≅ u ::: A0 | neA] -> 
-  [Γ0 |- t ≅ u ::: A0].
-Proof.
-  intros [] [? ? [] [] []].
-  do 2 eapply TermTrans.
-  all: mltt.
-Qed.
-
-Definition escapeEqTermPi {Γ A} : forall (ΠA: [Γ ||-Πr A]) t u,
-  [Γ ||-Π t ≅ u ::: A | ΠA] -> 
-  [Γ |- t ≅ u ::: A].
-Proof.
-  intros [? ? ? ? []] ? ? [? ? [] [] ? ? ?] ; cbn in *.
-  eapply (TermTrans (t' := nfL)).
-  1: mltt.
-  assert [Γ |- redPi ≅ A] by mltt.
-  eapply (TermTrans (t' := nfR)).
-  all: mltt.
-Qed.
-
-Definition escapeEqTerm0 {Γ t u A} (H : [Γ ||-< zero | A ]) :
-  [Γ ||-< zero | t ≅ u ::: A | H ] ->
-  [Γ |- t ≅ u::: A].
-Proof.
-  eapply (LR_rect0
-  (fun Γ A T T0 T1 H => forall t u,
-    [Γ ||-< zero | t ≅ u ::: A | Build_LRValid H] -> 
-    [Γ |- t ≅ u ::: A])).
-  all: eauto using escapeEqTermNe, escapeEqTermPi.
-Qed.
-
-Definition escapeEqTerm1 {Γ t u A} (H : [Γ ||-< one | A ]) :
-  [Γ ||-< one | t ≅ u ::: A | H ] ->
-  [Γ |- t ≅ u::: A].
-Proof.
-  eapply (LR_rect1'
-  (fun Γ A T T0 T1 H => forall t u,
-    [Γ ||-< zero | t ≅ u ::: A | Build_LRValid H] -> 
-    [Γ |- t ≅ u ::: A])
-  (fun Γ A T T0 T1 H => forall t u,
-    [Γ ||-< one | t ≅ u ::: A | Build_LRValid H] -> 
-    [Γ |- t ≅ u ::: A])).
-  all: cbn in *.
-  - intros.
-    now eapply (escapeEqTerm0 (LRbuild lr)).
-  - intros ? [] ? ? [] ; cbn in *.
-    do 2 eapply TermTrans.
+  eapply (LR_rect (fun l Γ A lr => forall t u, [Γ ||-< l > t ≅ u : A | lr] -> [Γ |- t ≅ u : A])).
+  - intros ? [] ? ? [[termL] [termR]] ; cbn in *.
+    eapply (TermTrans (t' := termL)).
+    1: mltt.
+    eapply (TermTrans (t' := termR)).
+    1: mltt.
+    eapply TermConv.
     all: mltt.
-  - eauto using escapeEqTermNe.
-  - eauto using escapeEqTermPi.
-  - eauto.
+  - intros ? ? ? [] ? ? [] ; cbn in *.
+    eapply (TermTrans (t' := termL)).
+    1: mltt.
+    eapply (TermTrans (t' := termR)).
+    1: mltt.
+    eapply TermConv.
+    all: mltt.
+  - intros ? ? ? [] _ _ _ ? ? [[termL] [termR]] ; cbn in *.
+    eapply (TermTrans (t' := termL)).
+    1: mltt.
+    eapply (TermTrans (t' := termR)).
+    1: mltt.
+    eapply TermConv.
+    all: mltt.
 Qed.
