theories/Notations.v
@@ -1,0 +1,105 @@
+(** Declarative Typing *)
+(* The context Γ is well-formed *)
+Reserved Notation "[   |- Γ ]" (at level 0, Γ at level 50).
+(* The type A is well-formed in Γ *)
+Reserved Notation "[ Γ |- A ]" (at level 0, Γ, A at level 50).
+(* The term t has type A in Γ *)
+Reserved Notation "[ Γ |- t : A ]" (at level 0, Γ, t, A at level 50).
+(* Types A and B are (declaratively) convertible in Γ *)
+Reserved Notation "[ Γ |- A ≅ B ]" (at level 0, Γ, A, B at level 50).
+(* Terms t and t' are (declaratively) convertible in Γ *)
+Reserved Notation "[ Γ |- t ≅ t' : A ]" (at level 0, Γ, t, t', A at level 50).
+(* Type A one-step weak-head reduces to type B in Γ *)
+
+(** Reductions *)
+Reserved Notation "[ Γ |- A ⇒ B ]" (at level 0, Γ, A, B at level 50).
+(* Term t one-step weak-head reduces to term u at type A in Γ *)
+Reserved Notation "[ Γ |- t ⇒ u : A ]" (at level 0, Γ, t, u, A at level 50).
+(* Type A multi-step weak-head reduces to type B in Γ *)
+Reserved Notation "[ Γ |- A ⇒* B ]" (at level 0, Γ, A, B at level 50).
+(* Term t multi-step weak-head reduces to term t' at type A in Γ *)
+Reserved Notation "[ Γ |- t ⇒* t' : A ]" (at level 0, Γ, t, t', A at level 50).
+(* Type A weak-head reduces in at least one step to type B in Γ *)
+Reserved Notation "[ Γ |- A ⇒⁺ B ]" (at level 0, Γ, A, B at level 50).
+(* Term t weak-head reduces in at least one step to term u at type A in Γ *)
+Reserved Notation "[ Γ |- t ⇒⁺ u : A ]" (at level 0, Γ, t, u, A at level 50).
+(* Type A weak-head normalizes to B in Γ, ie it multi-step reduces to the weak-head normal form B*)
+Reserved Notation "[ Γ |- A ↘ B ]" (at level 0, Γ, A, B at level 50).
+(* Term t weak-head normalizes to u at type A in Γ *)
+Reserved Notation "[ Γ |- t ↘ u : A ]" (at level 0, Γ, t, u, A at level 50).
+(* Types A and B are well-formed and convertible in Γ *)
+
+(** Extra typing conditions *)
+Reserved Notation "[ Γ |- A :≅: B ]" (at level 0, Γ, A, B at level 50).
+(* Terms t and u are well-typed and convertible at type A in Γ *)
+Reserved Notation "[ Γ |- t :≅: u : A ]" (at level 0, Γ, t, u, A at level 50).
+(* Type A and B are well-formed and A weak-head reduces to B in Γ *)
+Reserved Notation "[ Γ |- A :⇒*: B ]" (at level 0, Γ, A, B at level 50).
+(* Terms t and u have type A in Γ and t weak-head reduces to u *)
+Reserved Notation "[ Γ |- t :⇒*: u : A ]" (at level 0, Γ, t, u, A at level 50).
+
+(** Logical relation *)
+
+(* The universe is reducible in Γ, according to the kit K *)
+Reserved Notation "[ K | Γ ||-U ]" (at level 0, K, Γ at level 50).
+(* The type A is reducible as a product type in Γ according to the kit K *)
+Reserved Notation "[ K | Γ ||-Π A ]" (at level 0, K, Γ, A at level 50).
+(* The type A is reducible in Γ, according to the kit K *)
+Reserved Notation "[ K | Γ ||- A ]"  (at level 0, K, Γ, A at level 50).
+(* The types A and B are reducibly convertible in Γ, given the proof R than A is reducible, according to the kit K*)
+Reserved Notation "[ K | Γ ||- A ≅ B | R ]" (at level 0, K, Γ, A, B, R at level 50).
+(* The term t is reducible at type A in Γ, given the proof R than A is reducible, according to the kit K *)
+Reserved Notation "[ K | Γ ||- t : A | R ]"  (at level 0, K, Γ, t, A, R at level 50).
+(* The terms t and u are reducibly convertible at type A in Γ, given the proof R than A is reducible, according to the kit K *)
+Reserved Notation "[ K | Γ ||- t ≅ u : A | R ]" (at level 0, K, Γ, t, u, A, R at level 50).
+
+(* The types A and B are reducibly equal in Γ, according to the pack P for Γ and A *)
+Reserved Notation "[ P | Γ ||- A ≅ B ]" (at level 0, P, Γ, A, B at level 50).
+(* The term t is reducible at type A in Γ, according to the pack P *)
+Reserved Notation "[ P | Γ ||- t : A ]" (at level 0, P, Γ, t, A at level 50).
+(* The terms t and u are reducibly equal at type A in Γ, according to the pack P *)
+Reserved Notation "[ P | Γ ||- t ≅ u : A ]" (at level 0, P, Γ, t, u, A at level 50).
+
+(* Type level l is (strictly) smaller than type level l' *)
+Reserved Notation "l << l'" (at level 70, l' at next level).
+
+(* A is reducible as a neutral in Γ *)
+Reserved Notation "[ Γ ||-ne A ]" (at level 0, Γ, A at level 50).
+(* Type B is reducibly convertible to type A in Γ, given the proof neA that A is reducible as neutral *)
+Reserved Notation "[ Γ ||-ne A ≅ B | neA ]" (at level 0, Γ, A, B, neA at level 50).
+(* Term t is reducible at type A in Γ, given the proof neA that A is reducible as neutral *)
+Reserved Notation "[ Γ ||-ne t : A | neA ]" (at level 0, Γ, t, A, neA at level 50).
+(* Terms t and u are reducibly convertible at type A in Γ, given the proof neA that A is reducible as neutral *)
+Reserved Notation "[ Γ ||-ne t ≅ u : A | neA ]" (at level 0, Γ, t, u, A at level 50).
+
+(* The type U is reducible in Γ at level l *)
+Reserved Notation "[ Γ ||-U l ]" (at level 0, Γ, l at level 50).
+(* The type B is reducibly convertible to U *)
+Reserved Notation "[ Γ ||-U≅ B ]" (at level 0, Γ, B at level 50).
+(* The term t is reducible at the universe U, given the proof R that the universe is reducible and the kits rec at lower levels *)
+Reserved Notation "[ rec | Γ ||-U t :U | R ]" (at level 0, rec, Γ, t, R at level 50).
+(* The terms t and u are reducibly convertible at the universe U, given the same *)
+Reserved Notation "[ rec | Γ ||-U t ≅ u :U | R ]" (at level 0, rec, Γ, t, u, R at level 50).
+
+
+(* The type A has the packs of a reducible product type in Γ *)
+Reserved Notation "[ Γ ||-Πd A ]" (at level 0, Γ, A at level 50).
+(* The type B is reducibly convertible to A in Γ, given the reducibility pack ΠA *)
+Reserved Notation "[ Γ ||-Π A ≅ B | ΠA ]" (at level 0, Γ, A, B, ΠA at level 50).
+(* The term t is reducible at type A in Γ, given the reducibility pack ΠA *)
+Reserved Notation "[ Γ ||-Π t : A | ΠA ]" (at level 0, Γ, t, A, ΠA at level 50).
+(* The terms t and u are reducibly convertible at type A in Γ, given the reducibility pack ΠA *)
+Reserved Notation "[ Γ ||-Π t ≅ u : A | ΠA ]" (at level 0, Γ, t, u, A, ΠA at level 50).
+
+(* The universe is reducible in Γ at level l *)
+Reserved Notation "[ Γ ||-< l >U]" (at level 0, Γ, l at level 50).
+(* The type A is reducible as a product type in Γ at level l *)
+Reserved Notation "[ Γ ||-< l >Π  A ]" (at level 0, Γ, l, A at level 50).
+(* The type A is reducible in Γ at level l *)
+Reserved Notation "[ Γ ||-< l >  A ]" (at level 0, Γ, l, A at level 50).
+(* The types A and B are reducibly convertible in Γ at level l, given the proof R that A is reducible *)
+Reserved Notation "[ Γ ||-< l >  A ≅ B | R ]" (at level 0, Γ, l, A, B, R at level 50).
+(* The term t is reducible at type A and level l in Γ, given the proof R that A is reducible *)
+Reserved Notation "[ Γ ||-< l >  t : A | R ]" (at level 0, Γ, l, t, A, R at level 50).
+(* The terms t and u are reducibly convertible at type A and level l in Γ, given the proof R that A is reducible *)
+Reserved Notation "[ Γ ||-< l > t ≅ u : A | R ]" (at level 0, Γ, l, t, u, A, R at level 50).
