theories/Properties.v
@@ -1,5 +1,5 @@
 From MetaCoq.PCUIC Require Import PCUICAst.
-From LogRel Require Import Automation Untyped MLTTTyping.
+From LogRel Require Import Automation Notations Untyped MLTTTyping.
 
 Definition concons_inv {Γ na A} : [|- Γ,, vass na A] -> [|- Γ].
 Proof.
@@ -14,7 +14,7 @@ Qed.
 #[global] Hint Resolve concons_inv concons_inv': mltt.
 
 Definition WFterm {Γ} {t A} :
-    [ Γ |- t ::: A ] -> 
+    [ Γ |- t : A ] -> 
     [ |- Γ ].
 Proof.
   induction 1 ; mltt.
@@ -32,7 +32,7 @@ Qed.
 #[global] Hint Resolve WFtype : mltt.
 
 Definition WFEqTerm {Γ} {t u A} :
-    [ Γ |- t ≅ u ::: A ] -> 
+    [ Γ |- t ≅ u : A ] -> 
     [ |- Γ ].
 Proof.
     induction 1; mltt.
@@ -50,8 +50,8 @@ Qed.
 #[global] Hint Resolve WFEqType : mltt.
 
 Definition redFirstTerm {Γ t u A} : 
-  [ Γ |- t ⇒ u ::: A] ->
-  [ Γ |- t ::: A ].
+  [ Γ |- t ⇒ u : A] ->
+  [ Γ |- t : A ].
 Proof.
   induction 1 ; mltt.
 Qed.
@@ -68,8 +68,8 @@ Qed.
 #[global] Hint Resolve redFirst : mltt.
 
 Definition redFirstCTerm {Γ t u A} : 
-  [ Γ |- t ⇒* u ::: A] ->
-  [ Γ |- t ::: A ].
+  [ Γ |- t ⇒* u : A] ->
+  [ Γ |- t : A ].
 Proof.
   induction 1 ; mltt.
 Qed.
@@ -88,8 +88,8 @@ Qed.
 (*Removed the next two lemmas, as they are just projections…*)
 
 (* Definition redFirstCWFTerm {Γ t u A} : 
-  [ Γ |- t :⇒*: u ::: A] ->
-  [ Γ |- t ::: A ].
+  [ Γ |- t :⇒*: u : A] ->
+  [ Γ |- t : A ].
 Proof.
   now intros [].
 Qed. *)
