theories/Untyped.v
@@ -1,14 +1,17 @@
 From MetaCoq.PCUIC Require Import PCUICAst PCUICAstUtils PCUICNormal.
 From LogRel Require Import Automation.
 
+Definition U := (tSort Universe.type0).
+Definition eta_expand (f : term) := tApp (lift0 1 f) (tRel 0).
+
+#[global] Hint Transparent U : mltt.
+
 Notation whne := (whne RedFlags.default empty_global_env).
 Notation whnf := (whnf RedFlags.default empty_global_env).
 Definition emptyName : aname := 
   ltac:(repeat econstructor).
 
 #[global] Hint Constructors PCUICNormal.whne PCUICNormal.whnf : mltt.
-
-Definition eta {A B} (f : A -> B) : f = fun x => f x := eq_refl.
 
 Inductive isType Γ : term -> Type :=
   | ProdType {na A B} : isType Γ (tProd na A B)
@@ -28,6 +31,16 @@ Lemma isFun_whnf Γ t : isFun Γ t -> whnf Γ t.
 Proof.
   induction 1.
   all: now constructor.
+Qed.
+
+Lemma neU Γ : whne Γ U -> False.
+Proof.
+  intros H.
+  inversion H.
+  apply mkApps_nisApp in H0 as [? _].
+  1: unfold U in H0.
+  2: cbn.
+  all: congruence.
 Qed.
 
 Lemma nePi Γ na A B : whne Γ (tProd na A B) -> False.
